helping/HelpingAux.v
@@ -5,249 +5,37 @@ Require Import SchHeader SchI SchA.
 From CRIS.helping Require Import Header HelpingOn HelpingOff.
 
 (* This file contains auxilliary lemmas for proving HelpOn ≼ HelpOff. *)
-Section auxilliary.
-  Context {Σ : GRA}.
-
-  Lemma Red_vis_Assume {R} P (ktr : () → itree crisE R) :
-    ModTr.trans (vis (Events.Assume P) ktr) =
-    a <- itreeV_itree (ModTr.handle_Assume P);; ModTr.trans (ktr a).
-  Proof using. rewrite vis_trigger Red.bind Red.Assume; ss. Qed.
-
-  Lemma Red_vis_Take {R} X (ktr : X → itree crisE R) :
-    ModTr.trans (vis (Events.Take X) ktr) =
-    x <- trigger (Take X);; ModTr.trans (ktr x).
-  Proof using. rewrite /ModTr.trans interpV_vis /itreeV_itree /=. grind. Qed.
-
-  Lemma Red_unwrapUK {X R} x (ktr : X -> itree crisE R) :
-    ModTr.trans (unwrapUK x ktr) = unwrapUK x (fun x => ModTr.trans (ktr x)).
-  Proof using.
-    destruct x; ss.
-    eapply observe_eta; ss. f_equal. extensionality x. ss.
-  Qed.
-End auxilliary.
-
-Ltac replace_l :=
-  match goal with
-  | |- gpaco7 _ _ _ _ _ _ _ _ _ ?itr _ =>
-    pattern itr;
-    match goal with
-    | |- ?f ?a =>
-      refine (eq_ind_r f _ _); cycle 1
-    end
-  end.
-
-Ltac replace_r :=
-  match goal with
-  | |- gpaco7 _ _ _ _ _ _ _ _ _ _ ?itr =>
-    pattern itr;
-    match goal with
-    | |- ?f ?a =>
-      refine (eq_ind_r f _ _); cycle 1
-    end
-  end.
-
-Tactic Notation "red_LModTr" tactic(tac) :=
-  match goal with
-  | |- ?H => idtac H
-  end.
-
-Tactic Notation "red_ModTr" tactic(tac) :=
-  lazymatch goal with
-  | [ |- @ModTr.trans _ _ ?itr = _ ] =>
-      lazymatch itr with
-      | Ret _ =>
-          eapply Red.ret
-      | Tau _ =>
-          eapply Red.tau
-      | vis (Assume _) _ =>
-          eapply Red_vis_Assume
-      | vis (Take _) _ =>
-          eapply Red_vis_Take
-      | unwrapUK _ _ =>
-          eapply Red_unwrapUK
-      | _ =>
-          reflexivity
-      end
-  end.
-
-Tactic Notation "red_LModTr_state" tactic(tac) :=
-  lazymatch goal with
-  | [ |- @LModTr.interp_stateE ?A ?B ?itr ?state = _] =>
-    match itr with
-    | @iterV ?A ?B ?C ?handle ?itr => reflexivity
-    | _ =>
-      etransitivity;
-      [rewrite /= /LModTr.interp_stateE;
-        lazymatch itr with
-        | @ITree.bind _ _ _ _ _ =>
-          eapply interp_state_bind
-        | Ret _ =>
-          eapply interp_state_ret
-        | vis _ _ =>
-          etransitivity; [eapply interp_state_vis|tac; refl]
-        | Tau _ =>
-          eapply interp_state_tau
-        | unwrapUK _ _ =>
-          etransitivity; [rewrite /unwrapUK; refl|tac]
-        | _ =>
-          reflexivity
-        end
-      | fold (@LModTr.interp_stateE coreE); refl]
-    end
-  end.
-
-Ltac _gnorm_itr :=
-  lazymatch goal with
-  | [ |- Ret _ = _ ] =>
-      reflexivity
-  | [ |- Tau _ = _ ] =>
-      reflexivity
-  | [ |- vis _ _ = _ ] =>
-      reflexivity
-  | [ |- @ITree.bind ?E ?T ?U ?itr ?ktr = _ ] =>
-      etransitivity;
-      [ let itr' := fresh "itr" in cong (fun (itr' : itree E T) => @ITree.bind E T U itr' ktr); _gnorm_itr
-      | s; red_bind (do 1 _gnorm_itr) ]
-  | [ |- @SB.sandbox ?Σ ?R ?img ?imports ?scopes ?itr = _ ] =>
-      etransitivity;
-      [ cong (@SB.sandbox Σ R img imports scopes); _gnorm_itr | red_SB (do 1 _gnorm_itr) ]
-  | [ |- @SModTr.trans ?Σ ?sp ?R ?itr = _ ] =>
-      etransitivity;
-      [ cong (@SModTr.trans Σ sp R); _gnorm_itr | red_S (do 1 _gnorm_itr) ]
-  | [ |- @LModTr.interp_stateE ?E ?T ?itr ?st = _] =>
-      etransitivity;
-      [ cong (λ i, @LModTr.interp_stateE E T i st); _gnorm_itr | red_LModTr_state (do 1 _gnorm_itr)]
-  | [ |- @case_ _ _ _ _ _ _ _ _ _ _ _ ?E = _] =>
-      rewrite /case_ /LModTr.pure_state /=; _gnorm_itr
-  | [ |- @ModTr.trans ?A ?B ?itr = _] =>
-      etransitivity;
-      [ cong (@ModTr.trans A B); _gnorm_itr | red_ModTr (do 1 _gnorm_itr) ]
-  | [ |- @LModTr.handle_callE ?prog ?a = _] =>
-    rewrite /LModTr.handle_callE;
-    match goal with
-    | |- context [?a !! ?b] =>
-      pattern (a !! b);
-      match goal with
-      | |- ?f ?a =>
-        eapply (eq_ind_r f); cycle 1; [s; eapply (f_equal Some); _gnorm_itr|ss]
-      end
-    end
-  | [ |- trigger _ = _ ] =>
-      eapply trigger_vis
-  | [ |- assume _ = _ ] =>
-      eapply assume_assumeK
-  | [ |- guarantee _ = _ ] =>
-      eapply guarantee_guaranteeK
-  | [ |- unwrapU _ = _ ] =>
-      eapply unwrapU_unwrapUK
-  | [ |- unwrapN _ = _ ] =>
-      eapply unwrapN_unwrapNK
-  | [ |- RealUpdate _ _ = _ ] =>
-      eapply RealUpdate_RealUpdateK
-  | [ |- SModTr.HoareCall _ _ _ = _ ] =>
-      unfold SModTr.HoareCall;
-      _gnorm_itr
-  | [ |- fbody_trivial _ = _ ] =>
-      unfold fbody_trivial;
-      _gnorm_itr
-  | [ |- cput _ _ = _ ] =>
-      unfold cput;
-      _gnorm_itr
-  | [ |- cgetU _ = _ ] =>
-      unfold cgetU;
-      _gnorm_itr
-  | [ |- cgetN _ = _ ] =>
-      unfold cgetN;
-      _gnorm_itr
-  | [ |- cfunU _ _ = _ ] =>
-      unfold cfunU;
-      _gnorm_itr
-  | [ |- cfunN _ _ = _ ] =>
-      unfold cfunN;
-      _gnorm_itr
-  | [ |- ccallU _ _ = _ ] =>
-      unfold ccallU;
-      _gnorm_itr
-  | [ |- ccallN _ _ = _ ] =>
-      unfold ccallN;
-      _gnorm_itr
-  | [ |- triggerUB = _ ] =>
-      unfold triggerUB;
-      _gnorm_itr
-  | [ |- triggerNB = _ ] =>
-      unfold triggerNB;
-      _gnorm_itr
-  | [ |- ?itr = _ ] =>
-      reflexivity
-end.
-Ltac gnorm_itr :=
-etransitivity;
-[ _gnorm_itr
-| s;
-  lazymatch goal with
-  | [ |- Ret _ = _ ] =>
-      reflexivity
-  | [ |- Tau _ = _ ] =>
-      reflexivity
-  | [ |- vis _ _ = _ ] =>
-      eapply vis_trigger
-  | [ |- _ = _ ] =>
-      reflexivity
-  end
-].
-
-Ltac norm_l :=
-  replace_l; [s; gnorm_itr|].
-Ltac norm_r :=
-  replace_r; [s; gnorm_itr|].
-
-Ltac iter_l :=
-  replace_l; [rewrite unfold_iterV /itreeV_itree //|]; norm_l.
-Ltac iter_r :=
-  replace_r; [rewrite unfold_iterV /itreeV_itree //|]; norm_r.
-
-Ltac step_r := norm_r; guclo gsim_indC_spec; econs; instantiate (1:=smj_top).
-Ltac step_l := norm_l; guclo gsim_indC_spec; econs; instantiate (1:=smj_top).
-
-Ltac steps_r :=
-  norm_r; hrepeat (do 1 (guclo gsim_indC_spec; econs; instantiate (1:=smj_top); try norm_r)).
-Ltac steps_l :=
-  norm_l; hrepeat (do 1 (guclo gsim_indC_spec; econs; instantiate (1:=smj_top); try norm_l)).
-
-Ltac replace_tp_r :=
-  match goal with
-  | |- gpaco7 _ _ _ _ _ _ _ _ _ _ (LModTr.interp_stateE _ (iterV _ ?tp) _) =>
-      pattern tp;
-      match goal with
-      | |- ?f ?tp =>
-          eapply (eq_ind_r f); cycle 1
-      end
-  end.
-Ltac replace_tp_l :=
-  match goal with
-  | |- gpaco7 _ _ _ _ _ _ _ _ _ (LModTr.interp_stateE _ (iterV _ ?tp) _) _ =>
-      pattern tp;
-      match goal with
-      | |- ?f ?tp =>
-          eapply (eq_ind_r f); cycle 1
-      end
-  end.
-
 Notation "'⇓cris'" := (interpV (ModTr.handle_crisE)).
 Notation "'⇓sb(' m ')'" := (SB.sandbox m).
 Notation "'⇓smod(' sp ',' N ',' stid ')'" := (SModTr.trans sp N stid).
 
+Local Ltac gnorm_itr :=
+  match goal with
+  | |- context [?A] =>
+      match type of A with
+      | itree crisE Any.t => pattern A; eapply eq_ind; [|symmetry; hnorm_itr]
+      end
+  end.
+
+Ltac lookup_tac :=
+  match goal with
+  | H : ?l !! ?i = _ |- (_ <$> ?l) !! ?i = _ => rewrite list_lookup_fmap H //
+  | |- <[?i := _]> _ !! ?i = _ => rewrite list_lookup_insert; [|rewrite ?length_fmap //]
+  end.
+Ltac ghnorm_l := replace_l; [gnorm_itr; refl|].
+Ltac ghnorm_r := replace_r; [gnorm_itr; refl|].
+
 Section props.
   Context `{!crisG Γ Σ α β τ _S _I, !concG, !newschG}.
 
-  Lemma gsim_flag r g RR p_s p_t i_s i_t :
-    gpaco7 _gsim (cpn7 _gsim) r g (Any.t * Any.t)%type (Any.t * Any.t)%type RR smj_bot smj_bot
+  Lemma gsim_flag r g RR p_s p_t p_s1 p_t1 i_s i_t :
+    smj_le p_s1 p_s →
+    smj_le p_t1 p_t →
+    gpaco7 _gsim (cpn7 _gsim) r g (Any.t * Any.t)%type (Any.t * Any.t)%type RR p_s1 p_t1
       i_s i_t →
     gpaco7 _gsim (cpn7 _gsim) r g (Any.t * Any.t)%type (Any.t * Any.t)%type RR p_s p_t
       i_s i_t.
-  Proof.
-    intros ?; guclo flagC_spec; econs; try instantiate (1:=smj_bot); eauto using smj_le_bot.
-  Qed.
+  Proof using. guclo flagC_spec; econs; eauto. Qed.
 
   Lemma gsim_tau_src r g RR p_s p_t st_s itr_t prog_s tid_s tp_s k :
     tp_s !! tid_s = Some (⇓cris (tau;; k)) →
@@ -259,7 +47,7 @@ Section props.
     gpaco7 _gsim (cpn7 _gsim) r g (Any.t * Any.t)%type (Any.t * Any.t)%type RR p_s p_t
       (LModTr.interp_stateE Any.t (iterV (LModTr.handle_callE prog_s) (tid_s, tp_s)) st_s)
       itr_t.
-  Proof. intros Hi ?. giter_l. s. rewrite Hi; ss. gstep_l. gnorm_l. done. Qed.
+  Proof using. intros Hi ?. giter_l. s. rewrite Hi; ss. gstep_l. gnorm_l. done. Qed.
 
   Lemma gsim_tau_tgt r g RR p_s p_t itr_s st_t prog_t tid_t tp_t k :
     tp_t !! tid_t = Some (⇓cris (tau;; k)) →
@@ -271,71 +59,70 @@ Section props.
     gpaco7 _gsim (cpn7 _gsim) r g (Any.t * Any.t)%type (Any.t * Any.t)%type RR p_s p_t
       itr_s
       (LModTr.interp_stateE Any.t (iterV (LModTr.handle_callE prog_t) (tid_t, tp_t)) st_t).
-  Proof. intros Hi ?. giter_r; rewrite /= Hi; ss. gstep_r; gnorm_r. done. Qed.
+  Proof using. intros Hi ?. giter_r; rewrite /= Hi; ss. gstep_r; gnorm_r. done. Qed.
 
-  Lemma gsim_Choose_src r g RR p_s p_t st_s st_t prog_s prog_t tid_s tid_t tp_s tp_t
-      msk_c X k (k2 : Any.t → _) :
-    tp_s !! tid_s = Some (x <- ⇓cris (⇓sb(msk_c) (x <- trigger (Choose X);; k x));; k2 x) →
+  Lemma gsim_Choose_src r g RR p_s p_t st_s prog_s tid_s tp_s X k itr_t :
+    tp_s !! tid_s = Some (⇓cris (x <- trigger (Choose X);; k x)) →
     (∃ (x : X),
       gpaco7 _gsim (cpn7 _gsim) r g (Any.t * Any.t)%type (Any.t * Any.t)%type RR smj_top p_t
         (LModTr.interp_stateE Any.t
           (iterV (LModTr.handle_callE prog_s)
-            (tid_s, <[tid_s := (x <- ⇓cris (⇓sb(msk_c) (k x));; k2 x)]> tp_s)) st_s)
-        (LModTr.interp_stateE Any.t (iterV (LModTr.handle_callE prog_t) (tid_t, tp_t)) st_t)) →
+            (tid_s, <[tid_s := ⇓cris (k x)]> tp_s)) st_s)
+        itr_t) →
     gpaco7 _gsim (cpn7 _gsim) r g (Any.t * Any.t)%type (Any.t * Any.t)%type RR p_s p_t
       (LModTr.interp_stateE Any.t (iterV (LModTr.handle_callE prog_s) (tid_s, tp_s)) st_s)
-      (LModTr.interp_stateE Any.t (iterV (LModTr.handle_callE prog_t) (tid_t, tp_t)) st_t).
-  Proof.
-    rewrite -vis_trigger SBRed.vis; case_match; intros Hi [x Hk]; iter_l; rewrite Hi; ss.
-    { step_l. exists x; norm_l. steps_l. ired. done. }
-    { step_l. ss. }
+      itr_t.
+  Proof using.
+    intros Hi [x Hk]; giter_l; s; rewrite Hi /=; gstep_l; exists x; gsteps_l.
+    by (ired; eapply Hk).
   Qed.
 
-  Lemma gsim_Choose_tgt r g RR p_s p_t st_s st_t prog_s prog_t tid_s tid_t tp_s tp_t
-      msk_c X k (k2 : Any.t → _) :
-    msk_c _ (subevent _ (Choose X)) = true →
-    tp_t !! tid_t = Some (x <- ⇓cris (⇓sb(msk_c) (x <- trigger (Choose X);; k x));; k2 x) →
+  Lemma gsim_Choose_tgt r g RR p_s p_t st_t prog_t tid_t tp_t X k itr_s :
+    tp_t !! tid_t = Some (⇓cris (x <- trigger (Choose X);; k x)) →
     (∀ (x : X),
       gpaco7 _gsim (cpn7 _gsim) r g (Any.t * Any.t)%type (Any.t * Any.t)%type RR p_s smj_top
-        (LModTr.interp_stateE Any.t (iterV (LModTr.handle_callE prog_s) (tid_s, tp_s)) st_s)
+        itr_s
         (LModTr.interp_stateE Any.t
           (iterV (LModTr.handle_callE prog_t)
-            (tid_t, <[tid_t := (x <- ⇓cris (⇓sb(msk_c) (k x));; k2 x)]> tp_t)) st_t)) →
+            (tid_t, <[tid_t := ⇓cris (k x)]> tp_t)) st_t)) →
     gpaco7 _gsim (cpn7 _gsim) r g (Any.t * Any.t)%type (Any.t * Any.t)%type RR p_s p_t
-      (LModTr.interp_stateE Any.t (iterV (LModTr.handle_callE prog_s) (tid_s, tp_s)) st_s)
+      itr_s
       (LModTr.interp_stateE Any.t (iterV (LModTr.handle_callE prog_t) (tid_t, tp_t)) st_t).
-  Proof.
-    rewrite -vis_trigger SBRed.vis; case_match eqn:Hmsk2; intros Hmsk Hi Hk; ss.
-    { iter_r; rewrite Hi; ss. step_r. intros x. steps_r. ired. done. }
-    { rewrite Hmsk // in Hmsk2. }
+  Proof using.
+    intros Hi Hk; giter_r; s; rewrite Hi /=; gstep_r; intros x; gsteps_r.
+    by ired.
   Qed.
 
-  Lemma gsim_Take_src r g RR p_s p_t st_s st_t prog_s prog_t tid_s tid_t tp_s tp_t X k :
+  Lemma gsim_Take_src r g RR p_s p_t st_s prog_s tid_s tp_s X k itr_t :
     tp_s !! tid_s = Some (⇓cris (x <- trigger (Take X);; k x)) →
     (∀ (x : X),
       gpaco7 _gsim (cpn7 _gsim) r g (Any.t * Any.t)%type (Any.t * Any.t)%type RR smj_top p_t
         (LModTr.interp_stateE Any.t
           (iterV (LModTr.handle_callE prog_s)
             (tid_s, <[tid_s := ⇓cris (k x)]> tp_s)) st_s)
-        (LModTr.interp_stateE Any.t (iterV (LModTr.handle_callE prog_t) (tid_t, tp_t)) st_t)) →
+        itr_t) →
     gpaco7 _gsim (cpn7 _gsim) r g (Any.t * Any.t)%type (Any.t * Any.t)%type RR p_s p_t
       (LModTr.interp_stateE Any.t (iterV (LModTr.handle_callE prog_s) (tid_s, tp_s)) st_s)
-      (LModTr.interp_stateE Any.t (iterV (LModTr.handle_callE prog_t) (tid_t, tp_t)) st_t).
-  Proof. intros Hi ?; giter_l; s. rewrite Hi; ss. gstep_l; i; gstep_l; gnorm_l. ired; done. Qed.
+      itr_t.
+  Proof using.
+    intros Hi Hk; giter_l; s; rewrite Hi /=; gstep_l; intros x; gsteps_l.
+    by (ired).
+  Qed.
 
-  Lemma gsim_Take_tgt r g RR p_s p_t st_s st_t prog_s prog_t tid_s tid_t tp_s tp_t X k :
+  Lemma gsim_Take_tgt r g RR p_s p_t st_t prog_t tid_t tp_t X k itr_s :
     tp_t !! tid_t = Some (⇓cris (x <- trigger (Take X);; k x)) →
     (∃ (x : X),
       gpaco7 _gsim (cpn7 _gsim) r g (Any.t * Any.t)%type (Any.t * Any.t)%type RR p_s smj_top
-        (LModTr.interp_stateE Any.t (iterV (LModTr.handle_callE prog_s) (tid_s, tp_s)) st_s)
+        itr_s
         (LModTr.interp_stateE Any.t
           (iterV (LModTr.handle_callE prog_t)
-          (tid_t, <[tid_t := (⇓cris (k x))]> tp_t)) st_t)) →
+            (tid_t, <[tid_t := ⇓cris (k x)]> tp_t)) st_t)) →
     gpaco7 _gsim (cpn7 _gsim) r g (Any.t * Any.t)%type (Any.t * Any.t)%type RR p_s p_t
-      (LModTr.interp_stateE Any.t (iterV (LModTr.handle_callE prog_s) (tid_s, tp_s)) st_s)
+      itr_s
       (LModTr.interp_stateE Any.t (iterV (LModTr.handle_callE prog_t) (tid_t, tp_t)) st_t).
-  Proof.
-    intros Hi [x Hk]; ss. giter_r; rewrite /= Hi; ss. gstep_r. exists x. gstep_r. ired. done.
+  Proof using.
+    intros Hi [x Hk]; giter_r; s; rewrite Hi /=; gstep_r; exists x; gsteps_r.
+    by ired.
   Qed.
 
   Lemma gsim_Call_src r g RR p_s p_t st_s st_t prog_s prog_t tid_s tid_t tp_s tp_t fn args k :
@@ -348,7 +135,7 @@ Section props.
     gpaco7 _gsim (cpn7 _gsim) r g (Any.t * Any.t)%type (Any.t * Any.t)%type RR p_s p_t
       (LModTr.interp_stateE Any.t (iterV (LModTr.handle_callE prog_s) (tid_s, tp_s)) st_s)
       (LModTr.interp_stateE Any.t (iterV (LModTr.handle_callE prog_t) (tid_t, tp_t)) st_t).
-  Proof.
+  Proof using.
     intros Hi Hk.
     giter_l. rewrite /= Hi; ss. gstep_l. ired.
     replace_l; [|apply Hk].
@@ -369,7 +156,7 @@ Section props.
     gpaco7 _gsim (cpn7 _gsim) r g (Any.t * Any.t)%type (Any.t * Any.t)%type RR p_s p_t
       (LModTr.interp_stateE Any.t (iterV (LModTr.handle_callE prog_s) (tid_s, tp_s)) st_s)
       (LModTr.interp_stateE Any.t (iterV (LModTr.handle_callE prog_t) (tid_t, tp_t)) st_t).
-  Proof.
+  Proof using.
     intros Hi Hk.
     giter_r. rewrite /= Hi; ss. gstep_r. ired.
     replace_r; [|apply Hk].
@@ -391,7 +178,7 @@ Section props.
     gpaco7 _gsim (cpn7 _gsim) r g (Any.t * Any.t)%type (Any.t * Any.t)%type RR p_s p_t
       (LModTr.interp_stateE Any.t (iterV (LModTr.handle_callE prog_s) (tid_s, tp_s)) st_s)
       itr_t.
-  Proof.
+  Proof using.
     intros Hi Hk.
     giter_l. rewrite /= Hi; ss. gstep_l. ired.
     replace_l; [|apply Hk].
@@ -409,151 +196,140 @@ Section props.
     gpaco7 _gsim (cpn7 _gsim) r g (Any.t * Any.t)%type (Any.t * Any.t)%type RR p_s p_t
       (itr_s)
       (LModTr.interp_stateE Any.t (iterV (LModTr.handle_callE prog_t) (tid_t, tp_t)) st_t).
-  Proof.
+  Proof using.
     intros Hi Hk.
     giter_r. rewrite /= Hi; ss. gstep_r. ired.
     replace_r; [|apply Hk].
     do 1 f_equal. grind.
   Qed.
-  (* Lemma gsim_sGet_tgt r g RR p_s p_t st_s st_t prog_s prog_t tid_s tid_t tp_s tp_t
-      img_c msk_c scp_c key k (k2 : Any.t → _) r_t :
-    tp_t !! tid_t = Some (x <- ⇓cris (⇓sb(msk_c) (x <- trigger (SGet key);; k x));; k2 x) →
-    existsb (String.eqb key.1) scp_c →
-    (∃ t, alist_find key st_t = Some t ∧
-      gpaco7 _gsim (cpn7 _gsim) r g (Any.t * Any.t)%type (Any.t * Any.t)%type RR p_s smj_top
-        (LModTr.interp_stateE Any.t (iterV (LModTr.handle_callE prog_s) (tid_s, tp_s)) st_s)
-        (LModTr.interp_stateE Any.t
-          (iterV (LModTr.handle_callE prog_t)
-            (tid_t, <[tid_t := (x <- ⇓cris (⇓sb(msk_c) (k t));; k2 x)]> tp_t))
-          (Any.pair (ModTr.alist_encode st_t) r_t))) →
-    gpaco7 _gsim (cpn7 _gsim) r g (Any.t * Any.t)%type (Any.t * Any.t)%type RR p_s p_t
-      (LModTr.interp_stateE Any.t (iterV (LModTr.handle_callE prog_s) (tid_s, tp_s)) st_s)
-      (LModTr.interp_stateE Any.t (iterV (LModTr.handle_callE prog_t) (tid_t, tp_t))
-        (Any.pair (ModTr.alist_encode st_t) r_t)).
-  Proof.
-    intros Hin Hkey [t [Ht Hk]].
-    iter_r; rewrite Hin; ss.
-    rewrite Hkey /=.
-    norm_r. step_r. norm_r. hss. rewrite ModTr.alist_encode_decode Ht /=. ired. eapply Hk.
-  Qed.
 
-  Lemma gsim_sGet_src r g RR p_s p_t st_s st_t prog_s prog_t tid_s tid_t tp_s tp_t
-      img_c msk_c scp_c key k (k2 : Any.t → _) r_s :
-    tp_s !! tid_s = Some (x <- ⇓cris (⇓sb(img_c, msk_c, scp_c) (x <- trigger (SGet key);; k x));; k2 x) →
-    existsb (String.eqb key.1) scp_c →
-    (∃ t, alist_find key st_s = Some t ∧
-      gpaco7 _gsim (cpn7 _gsim) r g (Any.t * Any.t)%type (Any.t * Any.t)%type RR smj_top p_t
-        (LModTr.interp_stateE Any.t
-          (iterV (LModTr.handle_callE prog_s)
-            (tid_s, <[tid_s := (x <- ⇓cris (⇓sb(img_c, msk_c, scp_c) (k t));; k2 x)]> tp_s))
-          (Any.pair (ModTr.alist_encode st_s) r_s))
-        (LModTr.interp_stateE Any.t (iterV (LModTr.handle_callE prog_t) (tid_t, tp_t)) st_t)) →
-    gpaco7 _gsim (cpn7 _gsim) r g (Any.t * Any.t)%type (Any.t * Any.t)%type RR p_s p_t
-      (LModTr.interp_stateE Any.t (iterV (LModTr.handle_callE prog_s) (tid_s, tp_s))
-        (Any.pair (ModTr.alist_encode st_s) r_s))
-      (LModTr.interp_stateE Any.t (iterV (LModTr.handle_callE prog_t) (tid_t, tp_t)) st_t).
-  Proof.
-    intros Hin Hkey [t [Ht Hk]].
-    iter_l; rewrite Hin; ss.
-    rewrite Hkey /=.
-    norm_l. step_l. norm_l. hss. rewrite ModTr.alist_encode_decode Ht /=. ired. eapply Hk.
-  Qed.
-
-  Lemma gsim_s_cgetU_tgt r g RR p_s p_t st_s st_t prog_s prog_t tid_s tid_t tp_s tp_t b sp
-      img_c msk_c scp_c key {A} (k : A → _) (k2 : Any.t → _) r_t :
-    tp_t !! tid_t = Some (x <- ⇓cris (⇓sb(img_c, msk_c, scp_c)
-      (x <- ⇓smod(b, sp)(cgetU key);; k x));; k2 x) →
-    existsb (String.eqb key.1) scp_c →      
-    (∃ (t : A), alist_find key st_t = Some (t↑) ∧
-      gpaco7 _gsim (cpn7 _gsim) r g (Any.t * Any.t)%type (Any.t * Any.t)%type RR p_s smj_top
-        (LModTr.interp_stateE Any.t (iterV (LModTr.handle_callE prog_s) (tid_s, tp_s)) st_s)
-        (LModTr.interp_stateE Any.t
-          (iterV (LModTr.handle_callE prog_t)
-            (tid_t, <[tid_t := (x <- ⇓cris (⇓sb(img_c, msk_c, scp_c) (k t));; k2 x)]> tp_t))
-          (Any.pair (ModTr.alist_encode st_t) r_t))) →
-    gpaco7 _gsim (cpn7 _gsim) r g (Any.t * Any.t)%type (Any.t * Any.t)%type RR p_s p_t
-      (LModTr.interp_stateE Any.t (iterV (LModTr.handle_callE prog_s) (tid_s, tp_s)) st_s)
-      (LModTr.interp_stateE Any.t (iterV (LModTr.handle_callE prog_t) (tid_t, tp_t))
-        (Any.pair (ModTr.alist_encode st_t) r_t)).
-  Proof.
-    intros Hin Hkey [t [Ht Hk]].
-    iter_r; rewrite Hin /= Hkey /=.
-    norm_r. step_r. norm_r. hss. ired. rewrite ModTr.alist_encode_decode Ht /=. hss.
-    rewrite ?interpV_ret. ired. eauto.
-  Qed.
-
-  Lemma gsim_s_cgetU_src r g RR p_s p_t st_s st_t prog_s prog_t tid_s tid_t tp_s tp_t b sp
-      img_c msk_c scp_c key {A} (k : A → _) (k2 : Any.t → _) r_s :
-    tp_s !! tid_s = Some (x <- ⇓cris (⇓sb(img_c, msk_c, scp_c)
-      (x <- ⇓smod(b, sp)(cgetU key);; k x));; k2 x) →
-    existsb (String.eqb key.1) scp_c →      
-    (∃ t, alist_find key st_s = Some t↑ ∧
-      gpaco7 _gsim (cpn7 _gsim) r g (Any.t * Any.t)%type (Any.t * Any.t)%type RR smj_top p_t
-        (LModTr.interp_stateE Any.t
-          (iterV (LModTr.handle_callE prog_s)
-            (tid_s, <[tid_s := (x <- ⇓cris (⇓sb(img_c, msk_c, scp_c) (k t));; k2 x)]> tp_s))
-          (Any.pair (ModTr.alist_encode st_s) r_s))
-        (LModTr.interp_stateE Any.t (iterV (LModTr.handle_callE prog_t) (tid_t, tp_t)) st_t)) →
-    gpaco7 _gsim (cpn7 _gsim) r g (Any.t * Any.t)%type (Any.t * Any.t)%type RR p_s p_t
-      (LModTr.interp_stateE Any.t (iterV (LModTr.handle_callE prog_s) (tid_s, tp_s))
-        (Any.pair (ModTr.alist_encode st_s) r_s))
-      (LModTr.interp_stateE Any.t (iterV (LModTr.handle_callE prog_t) (tid_t, tp_t)) st_t).
-  Proof.
-    intros Hin Hkey [t [Ht Hk]].
-    iter_l; rewrite Hin /= Hkey; ss.
-    norm_l. step_l. norm_l. hss. ired. rewrite ModTr.alist_encode_decode Ht //=. hss.
-    rewrite ?interpV_ret. ired. done.
-  Qed.
-
-  Lemma gsim_s_cput_tgt r g RR p_s p_t st_s st_t prog_s prog_t tid_s tid_t tp_s tp_t b sp
-      img_c msk_c scp_c key {A} (v : A) (k : () → _) (k2 : Any.t → _) r_t :
-    tp_t !! tid_t = Some (x <- ⇓cris (⇓sb(img_c, msk_c, scp_c)
-      (x <- ⇓smod(b, sp)(cput key v);; k x));; k2 x) →
-    existsb (String.eqb key.1) scp_c →      
-    (gpaco7 _gsim (cpn7 _gsim) r g (Any.t * Any.t)%type (Any.t * Any.t)%type RR p_s smj_top
-      (LModTr.interp_stateE Any.t (iterV (LModTr.handle_callE prog_s) (tid_s, tp_s)) st_s)
-      (LModTr.interp_stateE Any.t
-        (iterV (LModTr.handle_callE prog_t)
-          (tid_t, <[tid_t := (x <- ⇓cris (⇓sb(img_c, msk_c, scp_c) (k ()));; k2 x)]> tp_t))
-        (Any.pair (ModTr.alist_encode (alist_upd key (v↑) st_t)) r_t))) →
-    gpaco7 _gsim (cpn7 _gsim) r g (Any.t * Any.t)%type (Any.t * Any.t)%type RR p_s p_t
-      (LModTr.interp_stateE Any.t (iterV (LModTr.handle_callE prog_s) (tid_s, tp_s)) st_s)
-      (LModTr.interp_stateE Any.t (iterV (LModTr.handle_callE prog_t) (tid_t, tp_t))
-        (Any.pair (ModTr.alist_encode st_t) r_t)).
-  Proof.
-    intros Hin Hkey Hk.
-    eapply lookup_lt_Some in Hin as Hlen.
-    iter_r; rewrite Hin /= Hkey /=. norm_r. step_r. norm_r. hss.
-    iter_r; rewrite list_lookup_insert //=.
-    norm_r. step_r. norm_r. rewrite list_insert_insert. ired.
-    rewrite ModTr.alist_encode_decode /=.
-    rewrite ?interpV_ret. ired. eauto.
-  Qed.
-
-  Lemma gsim_s_cput_src r g RR p_s p_t st_s st_t prog_s prog_t tid_s tid_t tp_s tp_t b sp
-      img_c msk_c scp_c key {A} (v : A) (k : () → _) (k2 : Any.t → _) r_s :
-    tp_s !! tid_s = Some (x <- ⇓cris (⇓sb(img_c, msk_c, scp_c)
-      (x <- ⇓smod(b, sp)(cput key v);; k x));; k2 x) →
-    existsb (String.eqb key.1) scp_c →      
+  Lemma gsim_GetTid_src r g RR p_s p_t itr_t st_s prog_s tid_s tp_s k :
+    tp_s !! tid_s = Some (⇓cris (x <- trigger GetTid;; k x)) →
     (gpaco7 _gsim (cpn7 _gsim) r g (Any.t * Any.t)%type (Any.t * Any.t)%type RR smj_top p_t
       (LModTr.interp_stateE Any.t
         (iterV (LModTr.handle_callE prog_s)
-          (tid_s, <[tid_s := (x <- ⇓cris (⇓sb(img_c, msk_c, scp_c) (k ()));; k2 x)]> tp_s))
-        (Any.pair (ModTr.alist_encode (alist_upd key (v↑) st_s)) r_s))
-      (LModTr.interp_stateE Any.t (iterV (LModTr.handle_callE prog_t) (tid_t, tp_t)) st_t)) →
+          (tid_s, <[tid_s := ⇓cris (k (tid_s))]> tp_s)) st_s)
+      itr_t) →
+    gpaco7 _gsim (cpn7 _gsim) r g (Any.t * Any.t)%type (Any.t * Any.t)%type RR p_s p_t
+      (LModTr.interp_stateE Any.t (iterV (LModTr.handle_callE prog_s) (tid_s, tp_s)) st_s)
+      itr_t.
+  Proof using. intros Hi Hk. giter_l. rewrite /= Hi; ss. gstep_l. by ired. Qed.
+
+  Lemma gsim_GetTid_tgt r g RR p_s p_t itr_s st_t prog_t tid_t tp_t k :
+    tp_t !! tid_t = Some (⇓cris (x <- trigger GetTid;; k x)) →
+    (gpaco7 _gsim (cpn7 _gsim) r g (Any.t * Any.t)%type (Any.t * Any.t)%type RR p_s smj_top
+      (itr_s)
+      (LModTr.interp_stateE Any.t
+        (iterV (LModTr.handle_callE prog_t)
+          (tid_t, <[tid_t := ⇓cris (k (tid_t))]> tp_t)) st_t)) →
+    gpaco7 _gsim (cpn7 _gsim) r g (Any.t * Any.t)%type (Any.t * Any.t)%type RR p_s p_t
+      (itr_s)
+      (LModTr.interp_stateE Any.t (iterV (LModTr.handle_callE prog_t) (tid_t, tp_t)) st_t).
+  Proof using. intros Hi Hk. giter_r. rewrite /= Hi; ss. gstep_r. by ired. Qed.
+
+  Lemma gsim_Yield_src r g RR p_s p_t itr_t st_s prog_s tid_s tid_s2 tp_s k :
+    tp_s !! tid_s = Some (⇓cris (x <- trigger (Yield tid_s2);; k x)) →
+    (gpaco7 _gsim (cpn7 _gsim) r g (Any.t * Any.t)%type (Any.t * Any.t)%type RR smj_top p_t
+      (LModTr.interp_stateE Any.t
+        (iterV (LModTr.handle_callE prog_s)
+          (tid_s2, <[tid_s := ⇓cris (k ())]> tp_s)) st_s)
+      itr_t) →
+    gpaco7 _gsim (cpn7 _gsim) r g (Any.t * Any.t)%type (Any.t * Any.t)%type RR p_s p_t
+      (LModTr.interp_stateE Any.t (iterV (LModTr.handle_callE prog_s) (tid_s, tp_s)) st_s)
+      itr_t.
+  Proof using. intros Hi Hk. giter_l. rewrite /= Hi; ss. gstep_l. by ired. Qed.
+
+  Lemma gsim_Yield_tgt r g RR p_s p_t itr_s st_t prog_t tid_t tid_t2 tp_t k :
+    tp_t !! tid_t = Some (⇓cris (x <- trigger (Yield tid_t2);; k x)) →
+    (gpaco7 _gsim (cpn7 _gsim) r g (Any.t * Any.t)%type (Any.t * Any.t)%type RR p_s smj_top
+      (itr_s)
+      (LModTr.interp_stateE Any.t
+        (iterV (LModTr.handle_callE prog_t)
+          (tid_t2, <[tid_t := ⇓cris (k ())]> tp_t)) st_t)) →
+    gpaco7 _gsim (cpn7 _gsim) r g (Any.t * Any.t)%type (Any.t * Any.t)%type RR p_s p_t
+      (itr_s)
+      (LModTr.interp_stateE Any.t (iterV (LModTr.handle_callE prog_t) (tid_t, tp_t)) st_t).
+  Proof using. intros Hi Hk. giter_r. rewrite /= Hi; ss. gstep_r. by ired. Qed.
+
+  Lemma gsim_SGet_tgt r g RR p_s p_t itr_s st_t prog_t tid_t tp_t key k r_t :
+    tp_t !! tid_t = Some (⇓cris (x <- trigger (SGet key);; k x)) →
+    map_Forall (const is_Some) st_t →
+    (gpaco7 _gsim (cpn7 _gsim) r g (Any.t * Any.t)%type (Any.t * Any.t)%type RR p_s smj_top
+      itr_s
+      (LModTr.interp_stateE Any.t
+        (iterV (LModTr.handle_callE prog_t)
+          (tid_t, <[tid_t := ⇓cris (k (default ()↑ (mjoin (st_t !! key))))]> tp_t))
+        (Any.pair (ModTr.state_encode st_t) r_t))) →
+    gpaco7 _gsim (cpn7 _gsim) r g (Any.t * Any.t)%type (Any.t * Any.t)%type RR p_s p_t
+      itr_s
+      (LModTr.interp_stateE Any.t (iterV (LModTr.handle_callE prog_t) (tid_t, tp_t))
+        (Any.pair (ModTr.state_encode st_t) r_t)).
+  Proof using.
+    intros Hin ? ?.
+    giter_r; rewrite /= Hin; ss. gsteps_r. hss. ired.
+    rewrite ModTr.state_encode_decode //.
+  Qed.
+
+  Lemma gsim_SGet_src r g RR p_s p_t itr_t st_s prog_s tid_s tp_s key k r_s :
+    tp_s !! tid_s = Some (⇓cris (x <- trigger (SGet key);; k x)) →
+    map_Forall (const is_Some) st_s →
+    (gpaco7 _gsim (cpn7 _gsim) r g (Any.t * Any.t)%type (Any.t * Any.t)%type RR smj_top p_t
+      (LModTr.interp_stateE Any.t
+        (iterV (LModTr.handle_callE prog_s)
+          (tid_s, <[tid_s := ⇓cris (k (default ()↑ (mjoin (st_s !! key))))]> tp_s))
+        (Any.pair (ModTr.state_encode st_s) r_s))
+      itr_t) →
     gpaco7 _gsim (cpn7 _gsim) r g (Any.t * Any.t)%type (Any.t * Any.t)%type RR p_s p_t
       (LModTr.interp_stateE Any.t (iterV (LModTr.handle_callE prog_s) (tid_s, tp_s))
-        (Any.pair (ModTr.alist_encode st_s) r_s))
-      (LModTr.interp_stateE Any.t (iterV (LModTr.handle_callE prog_t) (tid_t, tp_t)) st_t).
-  Proof.
-    intros Hin Hkey Hk.
-    eapply lookup_lt_Some in Hin as Hlen.
-    iter_l; rewrite Hin /= Hkey /=. norm_l. step_l. norm_l. hss.
-    iter_l; rewrite list_lookup_insert //=.
-    norm_l. step_l. norm_l. rewrite list_insert_insert. ired.
-    rewrite ModTr.alist_encode_decode /=.
-    rewrite ?interpV_ret. ired. eauto.
-  Qed. *)
+        (Any.pair (ModTr.state_encode st_s) r_s))
+      itr_t.
+  Proof using.
+    intros Hin ? ?.
+    giter_l; rewrite /= Hin; ss. gsteps_l. hss. ired.
+    rewrite ModTr.state_encode_decode //.
+  Qed.
+
+  Lemma gsim_SPut_tgt r g RR p_s p_t itr_s st_t prog_t tid_t tp_t key val k r_t :
+    tp_t !! tid_t = Some (⇓cris (x <- trigger (SPut key val);; k x)) →
+    map_Forall (const is_Some) st_t →
+    (gpaco7 _gsim (cpn7 _gsim) r g (Any.t * Any.t)%type (Any.t * Any.t)%type RR p_s smj_top
+      itr_s
+      (LModTr.interp_stateE Any.t
+        (iterV (LModTr.handle_callE prog_t)
+          (tid_t, <[tid_t := ⇓cris (k ())]> tp_t))
+        (Any.pair (ModTr.state_encode (<[key := Some val]> st_t)) r_t))) →
+    gpaco7 _gsim (cpn7 _gsim) r g (Any.t * Any.t)%type (Any.t * Any.t)%type RR p_s p_t
+      itr_s
+      (LModTr.interp_stateE Any.t (iterV (LModTr.handle_callE prog_t) (tid_t, tp_t))
+        (Any.pair (ModTr.state_encode st_t) r_t)).
+  Proof using.
+    intros Hin ? ?; eapply lookup_lt_Some in Hin as ?.
+    giter_r; rewrite /= Hin; ss. gsteps_r. hss.
+    rewrite ModTr.state_encode_decode //.
+    giter_r; rewrite /= list_lookup_insert //=. gsteps_r. ired.
+    rewrite list_insert_insert //.
+  Qed.
+
+  Lemma gsim_SPut_src r g RR p_s p_t itr_t st_s prog_s tid_s tp_s key val k r_s :
+    tp_s !! tid_s = Some (⇓cris (x <- trigger (SPut key val);; k x)) →
+    map_Forall (const is_Some) st_s →
+    (gpaco7 _gsim (cpn7 _gsim) r g (Any.t * Any.t)%type (Any.t * Any.t)%type RR smj_top p_t
+      (LModTr.interp_stateE Any.t
+        (iterV (LModTr.handle_callE prog_s)
+          (tid_s, <[tid_s := ⇓cris (k ())]> tp_s))
+        (Any.pair (ModTr.state_encode (<[key := Some val]> st_s)) r_s))
+      itr_t) →
+    gpaco7 _gsim (cpn7 _gsim) r g (Any.t * Any.t)%type (Any.t * Any.t)%type RR p_s p_t
+      (LModTr.interp_stateE Any.t (iterV (LModTr.handle_callE prog_s) (tid_s, tp_s))
+        (Any.pair (ModTr.state_encode st_s) r_s))
+      itr_t.
+  Proof using.
+    intros Hin ? ?; eapply lookup_lt_Some in Hin as ?.
+    giter_l; rewrite /= Hin; ss. gsteps_l. hss.
+    rewrite ModTr.state_encode_decode //.
+    giter_l; rewrite /= list_lookup_insert //=. gsteps_l. ired.
+    rewrite list_insert_insert //.
+  Qed.
 
   Lemma gsim_Assume_src r g RR p_s p_t st_s st_t prog_s prog_t tid_s tid_t tp_s tp_t k P r_s :
     tp_s !! tid_s = Some (⇓cris (x <- trigger (Assume P);; k x)) →
@@ -569,18 +345,18 @@ Section props.
       (LModTr.interp_stateE Any.t
         (iterV (LModTr.handle_callE prog_s) (tid_s, tp_s)) (Any.pair st_s (r_s↑)))
       (LModTr.interp_stateE Any.t (iterV (LModTr.handle_callE prog_t) (tid_t, tp_t)) st_t).
-  Proof.
+  Proof using.
     intros Hi Hk; pose proof Hi as Hlen; eapply lookup_lt_Some in Hlen.
-    iter_l; rewrite Hi; ss.
-    steps_l. hss. ired. hss. ired.
-    iter_l. rewrite list_lookup_insert //=. step_l. intros r_s2.
-      steps_l. ired. rewrite list_insert_insert.
-    iter_l. rewrite list_lookup_insert //=. step_l. intros Hr_s2.
-      steps_l. ired. rewrite list_insert_insert.
-    iter_l. rewrite list_lookup_insert //=. step_l.
-      steps_l. ired. hss. ired. rewrite list_insert_insert.
-    iter_l. rewrite list_lookup_insert //=. step_l.
-      steps_l. ired. rewrite list_insert_insert.
+    giter_l; rewrite /= Hi; ss.
+    gsteps_l. hss. ired. hss. ired.
+    giter_l. rewrite /= list_lookup_insert //=. gstep_l. intros r_s2.
+      gsteps_l. ired. rewrite list_insert_insert.
+    giter_l. rewrite /= list_lookup_insert //=. gstep_l. intros Hr_s2.
+      gsteps_l. ired. rewrite list_insert_insert.
+    giter_l. rewrite /= list_lookup_insert //=. gstep_l.
+      gsteps_l. ired. hss. ired. rewrite list_insert_insert.
+    giter_l. rewrite /= list_lookup_insert //=. gstep_l.
+      gsteps_l. ired. rewrite list_insert_insert.
     eapply Hk; done.
   Qed.
 
@@ -599,16 +375,16 @@ Section props.
         (iterV (LModTr.handle_callE prog_s) (tid_s, tp_s)) st_s)
       (LModTr.interp_stateE Any.t
         (iterV (LModTr.handle_callE prog_t) (tid_t, tp_t)) (Any.pair st_t (r_t↑))).
-  Proof.
+  Proof using.
     intros Hin [r_t2 [Hr_t2 Hk]]; pose proof Hin as Hlen; eapply lookup_lt_Some in Hlen.
-    iter_r; rewrite Hin /=. step_r. steps_r. hss. ired. hss. ired.
-    iter_r. rewrite list_lookup_insert //=. step_r. exists r_t2.
-      steps_r. rewrite list_insert_insert //=. ired.
-    iter_r. rewrite list_lookup_insert //=. step_r. unshelve eexists; eauto; ss.
-      steps_r. rewrite list_insert_insert //=. ired.
-    iter_r. rewrite list_lookup_insert //=. steps_r.
+    giter_r; rewrite /= Hin /=. gstep_r. gsteps_r. hss. ired. hss. ired.
+    giter_r. rewrite /= list_lookup_insert //=. gstep_r. exists r_t2.
+      gsteps_r. rewrite list_insert_insert //=. ired.
+    giter_r. rewrite /= list_lookup_insert //=. gstep_r. unshelve eexists; eauto; ss.
+      gsteps_r. rewrite list_insert_insert //=. ired.
+    giter_r. rewrite /= list_lookup_insert //=. gsteps_r.
       rewrite list_insert_insert //=. ired. hss. ired.
-    iter_r. rewrite list_lookup_insert //=. steps_r.
+    giter_r. rewrite /= list_lookup_insert //=. gsteps_r.
       rewrite list_insert_insert //=. ired. eauto.
   Qed.
 
@@ -626,7 +402,7 @@ Section props.
       (LModTr.interp_stateE Any.t
         (iterV (LModTr.handle_callE prog_s) (tid_s, tp_s)) (Any.pair st_s (r_s↑)))
       itr_t.
-  Proof.
+  Proof using.
     intros Hin Hk; pose proof Hin as Hlen; eapply lookup_lt_Some in Hlen.
     giter_l; rewrite /= Hin /=. gstep_l; ss. gnorm_l. hss. ired. hss. ired.
     giter_l; rewrite /= list_lookup_insert //=. gstep_l; ss.
@@ -651,7 +427,7 @@ Section props.
       itr_s
       (LModTr.interp_stateE Any.t
         (iterV (LModTr.handle_callE prog_s) (tid_t, tp_t)) (Any.pair st_t (r_t↑))).
-  Proof.
+  Proof using.
     intros Hin [Hval Hk]; pose proof Hin as Hlen; eapply lookup_lt_Some in Hlen.
     giter_r; rewrite /= Hin /=. gstep_r; ss. gnorm_r. hss. ired. hss. ired.
     giter_r; rewrite /= list_lookup_insert //=.
@@ -663,6 +439,284 @@ Section props.
     eapply Hk; done.
   Qed.
 
+  Lemma gsim_Guarantee_src r g RR p_s p_t st_s st_t prog_s prog_t tid_s tid_t tp_s tp_t k P r_s :
+    tp_s !! tid_s = Some (⇓cris (x <- trigger (Guarantee P);; k x)) →
+    (∃ r_s2,
+      ✓ r_s2 ∧ (Own r_s ⊢ |==> P ∗ Own r_s2) ∧
+      gpaco7 _gsim (cpn7 _gsim) r g (Any.t * Any.t)%type (Any.t * Any.t)%type RR smj_top p_t
+        (LModTr.interp_stateE Any.t
+          (iterV (LModTr.handle_callE prog_s)
+            (tid_s, <[tid_s := ⇓cris (k ())]> tp_s))
+          (Any.pair st_s (r_s2↑)))
+        (LModTr.interp_stateE Any.t (iterV (LModTr.handle_callE prog_t) (tid_t, tp_t)) st_t)) →
+    gpaco7 _gsim (cpn7 _gsim) r g (Any.t * Any.t)%type (Any.t * Any.t)%type RR p_s p_t
+      (LModTr.interp_stateE Any.t
+        (iterV (LModTr.handle_callE prog_s) (tid_s, tp_s)) (Any.pair st_s (r_s↑)))
+      (LModTr.interp_stateE Any.t (iterV (LModTr.handle_callE prog_t) (tid_t, tp_t)) st_t).
+  Proof using.
+    intros Hi [r_s2 Hk]; pose proof Hi as Hlen; eapply lookup_lt_Some in Hlen.
+    giter_l; rewrite /= Hi; ss.
+    gsteps_l. hss. ired. hss. ired.
+    giter_l. rewrite /= list_lookup_insert //=. gstep_l. exists r_s2.
+      gsteps_l. ired. rewrite list_insert_insert.
+    giter_l. rewrite /= list_lookup_insert //=. gstep_l. unshelve eexists; eauto.
+      gsteps_l. ired. rewrite list_insert_insert.
+    giter_l. rewrite /= list_lookup_insert //=. gstep_l.
+      gsteps_l. ired. hss. ired. rewrite list_insert_insert.
+    giter_l. rewrite /= list_lookup_insert //=. gstep_l.
+      gsteps_l. ired. rewrite list_insert_insert.
+    eauto.
+  Qed.
+
+  Lemma gsim_Guarantee_tgt r g RR p_s p_t st_s st_t prog_s prog_t tid_s tid_t tp_s tp_t k P r_t :
+    tp_t !! tid_t = Some (⇓cris (x <- trigger (Guarantee P);; k x)) →
+    (∀ r_t2,
+      ✓ r_t2 ∧ (Own r_t ⊢ |==> P ∗ Own r_t2) →
+      gpaco7 _gsim (cpn7 _gsim) r g (Any.t * Any.t)%type (Any.t * Any.t)%type RR p_s smj_top
+        (LModTr.interp_stateE Any.t (iterV (LModTr.handle_callE prog_s) (tid_s, tp_s)) st_s)
+        (LModTr.interp_stateE Any.t
+          (iterV (LModTr.handle_callE prog_t)
+            (tid_t, <[tid_t := ⇓cris (k ())]> tp_t))
+          (Any.pair st_t (r_t2↑)))) →
+    gpaco7 _gsim (cpn7 _gsim) r g (Any.t * Any.t)%type (Any.t * Any.t)%type RR p_s p_t
+      (LModTr.interp_stateE Any.t
+        (iterV (LModTr.handle_callE prog_s) (tid_s, tp_s)) st_s)
+      (LModTr.interp_stateE Any.t
+        (iterV (LModTr.handle_callE prog_t) (tid_t, tp_t)) (Any.pair st_t (r_t↑))).
+  Proof using.
+    intros Hin ?; pose proof Hin as Hlen; eapply lookup_lt_Some in Hlen.
+    giter_r; rewrite /= Hin /=. gstep_r. gsteps_r. hss. ired. hss. ired.
+    giter_r. rewrite /= list_lookup_insert //=. gstep_r. intros ?.
+      gsteps_r. rewrite list_insert_insert //=. ired.
+    giter_r. rewrite /= list_lookup_insert //=. gstep_r. i.
+      gsteps_r. rewrite list_insert_insert //=. ired.
+    giter_r. rewrite /= list_lookup_insert //=. gsteps_r.
+      rewrite list_insert_insert //=. ired. hss. ired.
+    giter_r. rewrite /= list_lookup_insert //=. gsteps_r.
+      rewrite list_insert_insert //=. ired.
+    eauto.
+  Qed.
+
+  (* HoareCall Lemmas *)
+  Definition fspec_option_meta (fspo : option fspec) : Type :=
+    match fspo with
+    | Some fsp => meta fsp
+    | None => unit
+    end.
+
+  Definition HoareCall_prologue fspo (varg : Any.t) N stid
+      : itree crisE (fspec_option_meta fspo * Any.t) :=
+    (match fspo as fspo return itree crisE (fspec_option_meta fspo * Any.t) with
+    | Some (fspec_mk pre post) =>
+        x <- trigger (Choose _);;
+        arg <- trigger (Choose Any.t);;
+        trigger (Guarantee (pre (N, stid) x varg arg));;;
+        Ret (x, arg)
+    | None => Ret (tt, varg)
+    end).
+
+  Definition HoareCall_epilogue fspo (x : fspec_option_meta fspo) (pret : Any.t) N stid
+      : itree crisE Any.t :=
+    (match fspo as fspo return fspec_option_meta fspo → itree crisE Any.t with
+    | Some (fspec_mk pre post) =>
+        λ x,
+          vret <- trigger (Take Any.t);;
+          trigger (Assume (post (N, stid) x vret pret));;;
+          Ret vret
+    | None => λ _, Ret pret
+    end) x.
+
+  Lemma HoareCall_unfold (sp : specmap) (fn : string) N stid :
+    SModTr.HoareCall (sp !! speckey_fn fn) fn ()↑ N stid =
+    xarg <- HoareCall_prologue (sp !! speckey_fn fn) (()↑) N stid;;
+    ret <- trigger (Call fn xarg.2);;
+    HoareCall_epilogue (sp !! speckey_fn fn) xarg.1 ret N stid.
+  Proof using.
+    rewrite /SModTr.HoareCall /HoareCall_prologue /HoareCall_epilogue; case_match; grind.
+  Qed.
+
+  Lemma gsim_HoareCall_prologue_both r g RR p_s p_t st_s st_t prog_s prog_t tid_s tid_t tp_s tp_t
+      scp fsp k_s k_t (res : Σ) arg N stid :
+    tp_s !! tid_s =
+      Some (⇓cris (x <- ⇓sb(msk_scp scp msk_true) (HoareCall_prologue fsp arg N stid);; k_s x)) →
+    tp_t !! tid_t =
+      Some (⇓cris (x <- ⇓sb(msk_scp scp msk_true) (HoareCall_prologue fsp arg N stid);; k_t x)) →
+    ✓ res →
+    (∀ (res1 : Σ) x, ✓ res1 →
+      gpaco7 _gsim (cpn7 _gsim) r g (Any.t * Any.t)%type (Any.t * Any.t)%type RR p_s p_t
+        (LModTr.interp_stateE Any.t (iterV (LModTr.handle_callE prog_s)
+          (tid_s, <[tid_s := ⇓cris (k_s x)]> tp_s))
+          (Any.pair st_s (res1↑)))
+        (LModTr.interp_stateE Any.t (iterV (LModTr.handle_callE prog_t)
+          (tid_t, <[tid_t := ⇓cris (k_t x)]> tp_t))
+          (Any.pair st_t (res1↑)))) →
+    gpaco7 _gsim (cpn7 _gsim) r g (Any.t * Any.t)%type (Any.t * Any.t)%type RR p_s p_t
+      (LModTr.interp_stateE Any.t
+        (iterV (LModTr.handle_callE prog_s) (tid_s, tp_s)) (Any.pair st_s (res↑)))
+      (LModTr.interp_stateE Any.t
+        (iterV (LModTr.handle_callE prog_t) (tid_t, tp_t)) (Any.pair st_t (res↑))).
+  Proof using.
+    rewrite /HoareCall_prologue.
+    intros Hin_s Hin_t Hres Hk.
+    eapply lookup_lt_Some in Hin_s as ?.
+    eapply lookup_lt_Some in Hin_t as ?.
+    destruct fsp as [[meta pre post] | ]; cycle 1.
+    { revert Hin_s; gnorm_itr; i; revert Hin_t; gnorm_itr; i.
+      specialize (Hk res ((), arg) Hres); revert Hk; rewrite ?list_insert_id //=.
+    }
+    eapply gsim_Choose_tgt; [rewrite Hin_t; do 2 f_equal; hnorm_itr|]. intros x.
+    eapply gsim_Choose_tgt; [lookup_tac; do 2 f_equal; hnorm_itr|].
+      intros varg. rewrite list_insert_insert. gnorm_r.
+    eapply gsim_Guarantee_tgt; [lookup_tac; do 2 f_equal; hnorm_itr|].
+      intros res2 Hres2. rewrite list_insert_insert. ghnorm_r.
+    eapply gsim_Choose_src; [rewrite Hin_s; do 2 f_equal; hnorm_itr|]. exists x.
+    eapply gsim_Choose_src; [lookup_tac; do 2 f_equal; hnorm_itr|].
+      exists varg. rewrite list_insert_insert. ghnorm_l.
+    eapply gsim_Guarantee_src; [lookup_tac; do 2 f_equal; hnorm_itr|].
+      exists res2; splits; try by des. rewrite list_insert_insert. ghnorm_l.
+    eapply gsim_flag; last eapply (Hk res2 (x, varg)).
+    { destruct p_s as [[|]|]; rr; ss; eauto. }
+    { destruct p_t as [[|]|]; rr; ss; eauto. }
+    by des.
+  Qed.
+
+  Lemma gsim_HoareCall_epilogue_both r g RR p_s p_t st_s st_t prog_s prog_t tid_s tid_t tp_s tp_t
+      scp fsp k_s k_t (res : Σ) x arg N stid :
+    tp_s !! tid_s =
+      Some (⇓cris (x <- ⇓sb(msk_scp scp msk_true) (HoareCall_epilogue fsp x arg N stid);; k_s x)) →
+    tp_t !! tid_t =
+      Some (⇓cris (x <- ⇓sb(msk_scp scp msk_true) (HoareCall_epilogue fsp x arg N stid);; k_t x)) →
+    ✓ res →
+    (∀ (res1 : Σ) x, ✓ res1 →
+      gpaco7 _gsim (cpn7 _gsim) r g (Any.t * Any.t)%type (Any.t * Any.t)%type RR p_s p_t
+        (LModTr.interp_stateE Any.t (iterV (LModTr.handle_callE prog_s)
+          (tid_s, <[tid_s := ⇓cris (k_s x)]> tp_s))
+          (Any.pair st_s (res1↑)))
+        (LModTr.interp_stateE Any.t (iterV (LModTr.handle_callE prog_t)
+          (tid_t, <[tid_t := ⇓cris (k_t x)]> tp_t))
+          (Any.pair st_t (res1↑)))) →
+    gpaco7 _gsim (cpn7 _gsim) r g (Any.t * Any.t)%type (Any.t * Any.t)%type RR p_s p_t
+      (LModTr.interp_stateE Any.t
+        (iterV (LModTr.handle_callE prog_s) (tid_s, tp_s)) (Any.pair st_s (res↑)))
+      (LModTr.interp_stateE Any.t
+        (iterV (LModTr.handle_callE prog_t) (tid_t, tp_t)) (Any.pair st_t (res↑))).
+  Proof using.
+    rewrite /HoareCall_epilogue.
+    intros Hin_s Hin_t Hres Hk.
+    eapply lookup_lt_Some in Hin_s as ?.
+    eapply lookup_lt_Some in Hin_t as ?.
+    destruct fsp as [[meta pre post] | ]; cycle 1.
+    { revert Hin_s; gnorm_itr; i; revert Hin_t; gnorm_itr; i.
+      specialize (Hk res (arg) Hres); revert Hk; rewrite ?list_insert_id //=.
+    }
+    eapply gsim_Take_src; [rewrite Hin_s; do 2 f_equal; hnorm_itr|]. intros varg.
+    eapply gsim_Take_tgt; [rewrite Hin_t; do 2 f_equal; hnorm_itr|]. exists varg.
+    eapply gsim_Assume_src; [lookup_tac; do 2 f_equal; hnorm_itr|].
+      intros res2 Hres2. rewrite list_insert_insert. gnorm_l.
+    eapply gsim_Assume_tgt; [lookup_tac; do 2 f_equal; hnorm_itr|].
+      exists res2; splits; try by des. rewrite list_insert_insert. ghnorm_l; ghnorm_r.
+    eapply gsim_flag; last eapply (Hk res2 (varg)).
+    { destruct p_s as [[|]|]; rr; ss; eauto. }
+    { destruct p_t as [[|]|]; rr; ss; eauto. }
+    by des.
+  Qed.
+
+  Lemma gsim_jobs_both {retID} r g RR st_s st_t prog_s prog_t tid_s tid_t tp_s tp_t
+      sp N stid k_s k_t (res : Σ) job mn :
+    tid_s < length tp_s →
+    tid_t < length tp_t →
+    ✓ res →
+    (∀ (res1 : Σ) (ret : retID), ✓ res1 →
+      gpaco7 _gsim (cpn7 _gsim) r g (Any.t * Any.t)%type (Any.t * Any.t)%type RR smj_bot smj_bot
+        (LModTr.interp_stateE Any.t (iterV (LModTr.handle_callE prog_s)
+          (tid_s, <[tid_s :=
+            ⇓cris (k_s ret)]> tp_s))
+          (Any.pair st_s (res1↑)))
+        (LModTr.interp_stateE Any.t (iterV (LModTr.handle_callE prog_t)
+          (tid_t, <[tid_t :=
+            ⇓cris (k_t ret)]> tp_t))
+          (Any.pair st_t (res1↑)))) →
+    gpaco7 _gsim (cpn7 _gsim) r g (Any.t * Any.t)%type (Any.t * Any.t)%type RR smj_bot smj_bot
+      (LModTr.interp_stateE Any.t (iterV (LModTr.handle_callE prog_s) (tid_s,
+        <[tid_s :=
+          ⇓cris (x <- ⇓sb(msk_scp (HelpingOn.scopes mn) msk_true) (⇓smod(sp, N, stid) (⇓sb(HelpingOn.msk_pure) job));; k_s x)]>
+        tp_s)) (Any.pair st_s (res↑)))
+      (LModTr.interp_stateE Any.t (iterV (LModTr.handle_callE prog_t) (tid_t,
+        <[tid_t :=
+          ⇓cris (x <- ⇓sb(msk_scp (HelpingOff.scopes mn) msk_true) (⇓smod(HelpingOn.sp mn sp, N, stid) (⇓sb(HelpingOn.msk_pure) job));; k_t x)]>
+        tp_t)) (Any.pair st_t (res↑))).
+  Proof using.
+    intros Hlen_s Hlen_t Hres Hk.
+    revert Hres Hk; generalize job res. clear job res.
+    gcofix CIH.
+    intros job res Hres Hk.
+    ides job.
+    { ghnorm_l; ghnorm_r.
+      eapply gpaco7_mon; eauto.
+    }
+    {
+      eapply gsim_tau_src; [rewrite list_lookup_insert //; do 2 f_equal; hnorm_itr|].
+      rewrite list_insert_insert.
+      eapply gsim_tau_tgt; [rewrite list_lookup_insert //; do 2 f_equal; hnorm_itr|].
+      rewrite list_insert_insert.
+      zprogress with smj_bot smj_bot _ _. gbase. eauto.
+    }
+    destruct e as [e|e]; rewrite !vis_trigger.
+    { destruct e as [P|res1|P].
+      { eapply gsim_Assume_src; [rewrite list_lookup_insert //; do 2 f_equal; hnorm_itr|].
+        intros res1 Hres1; rewrite list_insert_insert.
+        eapply gsim_Assume_tgt; [rewrite list_lookup_insert //; do 2 f_equal; hnorm_itr|].
+        exists res1; splits; (try by des); rewrite list_insert_insert.
+        ghnorm_l; ghnorm_r.
+        zprogress with smj_bot smj_bot _ _. gbase. eapply CIH; try by des.
+      }
+      { eapply gsim_AssumeRes_src; [rewrite list_lookup_insert //; do 2 f_equal; hnorm_itr|].
+        intros ?; rewrite list_insert_insert.
+        eapply gsim_AssumeRes_tgt; [rewrite list_lookup_insert //; do 2 f_equal; hnorm_itr|].
+        splits; (try by des); rewrite list_insert_insert.
+        ghnorm_l; ghnorm_r.
+        zprogress with smj_bot smj_bot _ _. gbase. eapply CIH; try by des.
+      }
+      { eapply gsim_Guarantee_tgt; [rewrite list_lookup_insert //; do 2 f_equal; hnorm_itr|].
+        intros res1 Hres1; rewrite list_insert_insert.
+        eapply gsim_Guarantee_src; [rewrite list_lookup_insert //; do 2 f_equal; hnorm_itr|].
+        exists res1; splits; (try by des); rewrite list_insert_insert.
+        ghnorm_l; ghnorm_r.
+        zprogress with smj_bot smj_bot _ _. gbase. eapply CIH; try by des.
+      }
+    }
+    destruct e as [e|e].
+    { ghnorm_l. ghnorm_l.
+      eapply gsim_Take_src; [rewrite list_lookup_insert //; do 2 f_equal; hnorm_itr|].
+      ss.
+    }
+    destruct e as [e|e].
+    { ghnorm_l. ghnorm_l.
+      eapply gsim_Take_src; [rewrite list_lookup_insert //; do 2 f_equal; hnorm_itr|].
+      ss.
+    }
+    destruct e as [X|X|I O fn args]; rewrite -!subevent_right !subevent_subevent.
+    { eapply gsim_Choose_tgt; [rewrite list_lookup_insert //; do 2 f_equal; hnorm_itr|].
+      intros x; rewrite list_insert_insert.
+      eapply gsim_Choose_src; [rewrite list_lookup_insert //; do 2 f_equal; hnorm_itr|].
+      exists x; rewrite list_insert_insert.
+      ghnorm_l; ghnorm_r.
+      zprogress with smj_bot smj_bot _ _. gbase. eapply CIH; try by des.
+    }
+    { eapply gsim_Take_src; [rewrite list_lookup_insert //; do 2 f_equal; hnorm_itr|].
+      intros x; rewrite list_insert_insert.
+      eapply gsim_Take_tgt; [rewrite list_lookup_insert //; do 2 f_equal; hnorm_itr|].
+      exists x; rewrite list_insert_insert.
+      ghnorm_l; ghnorm_r.
+      zprogress with smj_bot smj_bot _ _. gbase. eapply CIH; try by des.
+    }
+    { giter_l; giter_r.
+      rewrite /= ?list_lookup_insert //=. gnorm_l; gnorm_r.
+      gstep_l. instantiate (1:=smj_top).
+      intros ? ? <-. gsteps_l; gsteps_r. rewrite ?list_insert_insert. ired.
+      zprogress with smj_bot smj_bot _ _. gbase. eapply CIH; try by des.
+    }
+  Qed.
   (* Lemma gsim_Guarantee_src r g RR p_s p_t st_s st_t prog_s prog_t tid_s tid_t tp_s tp_t
       img_c msk_c scp_c k (k_2 : Any.t → _) r_s P :
     tp_s !! tid_s =
@@ -678,17 +732,17 @@ Section props.
       (LModTr.interp_stateE Any.t
         (iterV (LModTr.handle_callE prog_s) (tid_s, tp_s)) (Any.pair st_s (r_s↑)))
       (LModTr.interp_stateE Any.t (iterV (LModTr.handle_callE prog_t) (tid_t, tp_t)) st_t).
-  Proof.
+  Proof using.
     intros Hin [r_s2 [Hr_s2 Hk]]; pose proof Hin as Hlen; eapply lookup_lt_Some in Hlen.
     iter_l; rewrite Hin; ss.
-    step_l; ss. norm_l. hss. ired. hss. ired.
-    iter_l. rewrite list_lookup_insert //=. step_l. exists r_s2. step_l. norm_l.
+    step_l; ss. gnorm_l. hss. ired. hss. ired.
+    iter_l. rewrite list_lookup_insert //=. step_l. exists r_s2. step_l. gnorm_l.
     rewrite list_insert_insert //=. ired.
-    iter_l. rewrite list_lookup_insert //=. step_l. unshelve eexists; eauto. step_l. norm_l.
+    iter_l. rewrite list_lookup_insert //=. step_l. unshelve eexists; eauto. step_l. gnorm_l.
     rewrite list_insert_insert //=. ired.
-    iter_l. rewrite list_lookup_insert //=. step_l. norm_l.
+    iter_l. rewrite list_lookup_insert //=. step_l. gnorm_l.
     rewrite list_insert_insert //=. ired. hss. ired.
-    iter_l. rewrite list_lookup_insert //=. step_l. norm_l.
+    iter_l. rewrite list_lookup_insert //=. step_l. gnorm_l.
     rewrite list_insert_insert //=. ired.
     eapply Hk; done.
   Qed.
@@ -709,17 +763,17 @@ Section props.
       (LModTr.interp_stateE Any.t
         (iterV (LModTr.handle_callE prog_t) (tid_t, tp_t))
         (Any.pair st_t (r_t↑))).
-  Proof.
+  Proof using.
     intros Hin Hk; pose proof Hin as Hlen; eapply lookup_lt_Some in Hlen.
     iter_r; rewrite Hin; ss.
-    step_r; ss. norm_r. hss. ired. hss. ired.
-    iter_r. rewrite list_lookup_insert //=. step_r. intros r_t2. norm_r. step_r. norm_r.
+    step_r; ss. gnorm_r. hss. ired. hss. ired.
+    iter_r. rewrite list_lookup_insert //=. step_r. intros r_t2. gnorm_r. step_r. gnorm_r.
     rewrite list_insert_insert //=. ired.
-    iter_r. rewrite list_lookup_insert //=. step_r. intros Hr_t2. step_r. norm_r.
+    iter_r. rewrite list_lookup_insert //=. step_r. intros Hr_t2. step_r. gnorm_r.
     rewrite list_insert_insert //=. ired.
-    iter_r. rewrite list_lookup_insert //=. step_r. norm_r.
+    iter_r. rewrite list_lookup_insert //=. step_r. gnorm_r.
     rewrite list_insert_insert //=. ired. hss. ired.
-    iter_r. rewrite list_lookup_insert //=. step_r. norm_r.
+    iter_r. rewrite list_lookup_insert //=. step_r. gnorm_r.
     rewrite list_insert_insert //=. ired.
     apply Hk; done.
   Qed. *)
@@ -728,7 +782,7 @@ Section props.
 
   Lemma HoareCall_prologue_sred img_c fsp arg :
     ⇓smod(img_c, sp) (HoareCall_prologue fsp arg) = HoareCall_prologue fsp arg.
-  Proof.
+  Proof using.
     rewrite /HoareCall_prologue; unseal "Help"; destruct fsp as [[fsp | fsp] |].
     { repeat (rewrite interpV_bind interpV_trigger /=; grind).
       rewrite interpV_ret //.
@@ -739,7 +793,7 @@ Section props.
 
   Lemma HoareCall_epilogue_sred img_c fsp arg x :
     ⇓smod(img_c, sp) (HoareCall_epilogue fsp x arg) = HoareCall_epilogue fsp x arg.
-  Proof.
+  Proof using.
     rewrite /HoareCall_epilogue; unseal "Help"; destruct fsp as [[fsp | fsp] |].
     { repeat (rewrite interpV_bind interpV_trigger /=; grind).
       rewrite interpV_ret //.
@@ -750,7 +804,7 @@ Section props.
 
   Lemma HoareFun_prologue_sred img_c fsp arg :
     ⇓smod(img_c, sp) (HoareFun_prologue fsp arg) = HoareFun_prologue fsp arg.
-  Proof.
+  Proof using.
     rewrite /HoareFun_prologue; unseal "Help"; destruct fsp as [[fsp | fsp] |].
     { repeat (rewrite interpV_bind interpV_trigger /=; grind).
       rewrite interpV_ret //.
@@ -761,7 +815,7 @@ Section props.
 
   Lemma HoareFun_epilogue_sred img_c fsp arg x :
     ⇓smod(img_c, sp) (HoareFun_epilogue fsp x arg) = HoareFun_epilogue fsp x arg.
-  Proof.
+  Proof using.
     rewrite /HoareFun_epilogue; unseal "Help"; destruct fsp as [[fsp | fsp] |].
     { repeat (rewrite interpV_bind interpV_trigger /=; grind).
       rewrite interpV_ret //.
@@ -790,7 +844,7 @@ Section props.
         (iterV (LModTr.handle_callE prog_s) (tid_s, tp_s)) (Any.pair st_s (res↑)))
       (LModTr.interp_stateE Any.t
         (iterV (LModTr.handle_callE prog_t) (tid_t, tp_t)) (Any.pair st_t (res↑))).
-  Proof.
+  Proof using.
     intros Hin_s Hin_t Hres Hk.
     pose proof Hin_s as Hlen_s; eapply lookup_lt_Some in Hlen_s.
     pose proof Hin_t as Hlen_t; eapply lookup_lt_Some in Hlen_t.
@@ -801,7 +855,7 @@ Section props.
       specialize (Hk res ((), arg) Hres); revert Hk; rewrite ?list_insert_id //=.
     }
     { iter_l; iter_r; rewrite Hin_s Hin_t /HoareCall_prologue; unseal "Help". ss.
-      step_r; intros fsp2; step_l; exists fsp2. step_l; step_r. norm_l; norm_r. ired.
+      step_r; intros fsp2; step_l; exists fsp2. step_l; step_r. gnorm_l; gnorm_r. ired.
       eapply gsim_Choose_tgt; [rewrite list_lookup_insert; grind|]. intros varg.
       rewrite list_insert_insert.
       eapply gsim_Choose_src; [rewrite list_lookup_insert; grind|]. exists varg.
@@ -839,7 +893,7 @@ Section props.
         (iterV (LModTr.handle_callE prog_s) (tid_s, tp_s)) (Any.pair st_s (res↑)))
       (LModTr.interp_stateE Any.t
         (iterV (LModTr.handle_callE prog_t) (tid_t, tp_t)) (Any.pair st_t (res↑))).
-  Proof.
+  Proof using.
     intros Hin_s Hin_t Hres Hk.
     pose proof Hin_s as Hlen_s; eapply lookup_lt_Some in Hlen_s.
     pose proof Hin_t as Hlen_t; eapply lookup_lt_Some in Hlen_t.
@@ -889,7 +943,7 @@ Section props.
         (iterV (LModTr.handle_callE prog_s) (tid_s, tp_s)) (Any.pair st_s (res↑)))
       (LModTr.interp_stateE Any.t
         (iterV (LModTr.handle_callE prog_t) (tid_t, tp_t)) (Any.pair st_t (res↑))).
-  Proof.
+  Proof using.
     intros Hin_s Hin_t Hres Hk.
     pose proof Hin_s as Hlen_s; eapply lookup_lt_Some in Hlen_s.
     pose proof Hin_t as Hlen_t; eapply lookup_lt_Some in Hlen_t.
@@ -903,8 +957,8 @@ Section props.
     }
     { iter_l; iter_r; rewrite Hin_s Hin_t /HoareCall_epilogue /HoareFun_prologue; unseal "Help".
       ss.
-      step_l. intros varg. norm_l. step_l. norm_l. ired.
-      step_r. exists x. norm_r. step_r. norm_r. ired.
+      step_l. intros varg. gnorm_l. step_l. gnorm_l. ired.
+      step_r. exists x. gnorm_r. step_r. gnorm_r. ired.
       eapply gsim_Take_tgt; [rewrite list_lookup_insert //|exists varg; split; first eauto].
       rewrite list_insert_insert.
 
@@ -943,7 +997,7 @@ Section props.
         (iterV (LModTr.handle_callE prog_s) (tid_s, tp_s)) (Any.pair st_s (res↑)))
       (LModTr.interp_stateE Any.t
         (iterV (LModTr.handle_callE prog_t) (tid_t, tp_t)) (Any.pair st_t (res↑))).
-  Proof.
+  Proof using.
     intros Hin_s Hin_t Hres Hk.
     pose proof Hin_s as Hlen_s; eapply lookup_lt_Some in Hlen_s.
     pose proof Hin_t as Hlen_t; eapply lookup_lt_Some in Hlen_t.
@@ -957,8 +1011,8 @@ Section props.
     }
     { iter_l; iter_r; rewrite Hin_s Hin_t /HoareCall_prologue /HoareFun_epilogue; unseal "Help".
       ss.
-      step_r. intros vret. norm_r. step_r. norm_r. ired.
-      step_l. exists x. norm_l. step_l. norm_l. ired.
+      step_r. intros vret. gnorm_r. step_r. gnorm_r. ired.
+      step_l. exists x. gnorm_l. step_l. gnorm_l. ired.
       eapply gsim_Choose_src; [rewrite list_lookup_insert //|exists vret; split; first eauto].
       rewrite list_insert_insert.
 
@@ -996,7 +1050,7 @@ Section props.
         <[tid_t :=
           x <- ⇓cris (⇓sb(img_c, msk_c, scp_c) (⇓smod(img_c', sp) (x <- Helping.trans job;; k_t x)));; k_t1 x]>
         tp_t)) (Any.pair st_t (res↑))).
-  Proof.
+  Proof using.
     intros Hlen_s Hlen_t Hres Hk.
     apply gsim_flag.
     revert Hres; generalize job res. clear job res.
@@ -1096,10 +1150,10 @@ Section props.
         }
         { iter_l. rewrite list_lookup_insert //=.
           iter_r. rewrite list_lookup_insert //=.
-          norm_l; norm_r.
+          gnorm_l; gnorm_r.
           guclo gsim_indC_spec; econs; instantiate (1:=smj_top).
           intros ?? ->.
-          step_l; step_r. norm_l; norm_r. rewrite ?list_insert_insert. ired.
+          step_l; step_r. gnorm_l; gnorm_r. rewrite ?list_insert_insert. ired.
           zprogress.
           apply gsim_flag.
           gbase. eapply CIH; eauto using list_lookup_insert.
