helping/HelpingOff.v
@@ -1,19 +1,19 @@
 Require Import CRIS SchHeader.
-From CRIS.helping Require Import Header.
+From CRIS.helping Require Import Header HelpingOn.
 
 Module HelpingOff. Section HelpingOff.
   Context `{!crisG Γ Σ α β τ _S _I, !concG}.
 
   Context (mn : string).
   Context {jobID retID : Type}.
-  Context (jobcode : jobID → itree Helping.pureE retID).
+  Context (jobcode : jobID → itree crisE retID).
 
   Definition scopes : gmultiset string := {[+mn+]}.
 
   Definition run : Any.t → itree crisE Any.t :=
     λ arg,
       'jid : jobID <- arg↓?;;
-      𝒴;;; ret <- Helping.trans (jobcode jid);;
+      𝒴;;; ret <- SB.sandbox (HelpingOn.msk_pure) (jobcode jid);;
       𝒴;;; Ret ret↑.
 
   Definition help : Any.t → itree crisE Any.t :=
@@ -21,7 +21,8 @@ Module HelpingOff. Section HelpingOff.
       
   Definition fnsems : gmap (option string) (option (emask * (option fspec * fbody))) :=
     {[Some (Helping.run mn) := Some (msk_scp scopes msk_true, (Some fspec_trivial, run));
-      Some (Helping.help mn) := Some (msk_scp scopes msk_true, (Some fspec_trivial, help))]}.
+      Some (Helping.help mn) := Some (msk_scp scopes msk_true, (Some fspec_trivial, help));
+      Some (Helping.yield mn) := Some (msk_scp scopes msk_true, (None, fbody_trivial))]}.
 
   Program Definition Mod : SMod.t := {|
     SMod.scopes := scopes;
